restructured proof of refinement rule

src/temporal_logic/refinement.lean
@@ -1,5 +1,6 @@
 
 import temporal_logic.fairness
+import temporal_logic.pair
 import temporal_logic.lemmas
 
 universe variables u u₀ u₁ u₂
@@ -7,46 +8,17 @@ open predicate nat
 
 variables {α : Sort u₀} {β : Type u₁} {γ : Sort u₂}
 
+local attribute [-simp] or.comm or.left_comm or.assoc and.comm and.left_comm and.assoc
+
 namespace temporal
-
-section pair
-
-variables {α' : Type u} {β' : Type u₀} {γ' : Type u₁}
-variables (x : tvar α') (y : tvar β') (z : tvar γ')
-
-def pair : tvar (α' × β') :=
-lifted₂ prod.mk x y
-
-notation `⦃` x `,` l:(foldl `,` (h t, pair h t) x `⦄`)  := l
-
-@[simp]
-lemma pair_model (i : ℕ) :
-i ⊨ ⦃x,y⦄ = (i ⊨ y,i ⊨ x) :=
-by { cases x, cases y, refl }
-
-@[reducible]
-def pair.fst : var (α' × β') α' :=
-↑(@prod.fst α' β')
-
-@[simp]
-def pair.fst_mk (x : tvar α') (y : tvar β')
-: pair.fst ;; ⦃y,x⦄ = x :=
-by lifted_pred
-
--- @[simp]
-def pair.fst_mk' (x : tvar α') (y : tvar β')
-: ↑(@prod.fst α' β') ;; ⦃y,x⦄ = x :=
-pair.fst_mk _ _
-
-end pair
 
 namespace simulation
 section
 
 parameters {α' : Type u} {β' : Type u₀} {γ' : Type u₁ }
-parameters {p : pred' (α'×γ')} {q : pred' (β'×γ')}
-parameters {A : act (α'×γ')} {C : act (β'×γ')}
-parameters {J : pred' (α'×β'×γ')}
+parameters (p : pred' (α'×γ')) (q : pred' (β'×γ'))
+parameters (A : act (α'×γ')) (C : act (β'×γ'))
+parameters (J : pred' (α'×β'×γ'))
 
 variables (x : tvar α') (y : tvar β') (z : tvar γ')
 
@@ -58,10 +30,10 @@ def SPEC₁ (v : tvar β') (o : tvar γ') : cpred :=
 q ;; ⦃ o,v ⦄ ⋀
 ◻⟦ ⦃o,v⦄ <> C ⟧
 
-parameter [inhabited α']
+parameters [inhabited α']
 parameter SIM₀ : ∀ v o, (v,o) ⊨ q → ∃ w, (w,o) ⊨ p ∧ (w,v,o) ⊨ J
 parameter SIM
-: ∀ {w v o} v' o',
+: ∀ w v o v' o',
   (w,v,o) ⊨ J →
   C (v,o) (v',o') →
   ∃ w', A (w,o) (w',o') ∧
@@ -69,87 +41,93 @@ parameter SIM
 
 parameters (v : tvar β') (o : tvar γ')
 
-parameters {Γ : cpred}
-parameters H : Γ ⊢ SPEC₁ v o
-
 section witness
-variables (i : ℕ) (Hi : i ⊨ Γ)
-include H Hi
+variables (i : ℕ)
 
 open classical
 
-private noncomputable def ww : Π j : ℕ, { w : α' // j ≥ i → (w,j ⊨ v,j ⊨ o) ⊨ J }
- | j :=
-if h : j > i then
-     have h₀ : j ≥ 1,
-       by { apply succ_le_of_lt,
-            apply nat.lt_of_le_of_lt (nat.zero_le i) h },
-     have h₁ : i ≤ j - 1,
-       by { rw ← add_le_to_le_sub _ ; assumption },
-     have Hdec : j - 1 < j,
-       by { apply nat.sub_lt_of_pos_le, apply zero_lt_one,
-            assumption },
-     let hw := (ww (j-1)).property h₁ in
-     have Hstep : C (j - 1 ⊨ v, j - 1 ⊨ o) (j ⊨ v, j ⊨ o),
-       begin
-         clear_except H Hi h₀ h₁ h, replace H := (H.apply _ Hi).right ((j-1) - i),
-         simp at H, rw [← nat.add_sub_assoc,nat.add_sub_cancel_left,← succ_sub] at H
-         ; apply H <|> assumption,
-       end,
-     let x := some (SIM (j ⊨ v) (j ⊨ o) hw Hstep) in
-     have h₁ : j ≥ i → (x, j ⊨ v, j ⊨ o) ⊨ J,
-       from assume _, (some_spec (SIM (j ⊨ v) (j ⊨ o) hw Hstep)).right,
-     ⟨x,h₁⟩
-else if h' : i ≤ j then
-     have h : i = j,
-       by { apply le_antisymm h', apply le_of_not_gt, assumption },
-     have h₀ : (j ⊨ v, j ⊨ o) ⊨ q,
-          begin
-            clear_except H Hi h,
-            have := H.left.apply _ Hi, simp at this,
-            subst i, apply this,
-          end,
-     let x₀ := some (SIM₀ (j ⊨ v) (j ⊨ o) h₀) in
-     have h₁ : j ≥ i → (x₀, j ⊨ v, j ⊨ o) ⊨ J,
-       from assume _, (some_spec (SIM₀ (j ⊨ v) (j ⊨ o) h₀)).right,
-     ⟨x₀,h₁⟩
-else
-  have h₁ : j ≥ i → (default α', j ⊨ v, j ⊨ o) ⊨ J,
-    by { intro, exfalso, apply h', assumption, },
-  ⟨default α',h₁⟩
+private noncomputable def w : ℕ → α'
+ | 0 := (ε w', (w',i ⊨ o) ⊨ p ∧ (w', i ⊨ v, i ⊨ o) ⊨ J)
+ | (succ j) := (ε w', A (w j,i+j ⊨ o) (w',i + succ j ⊨ o) ∧
+                      (w', i + succ j ⊨ v, i + succ j ⊨ o) ⊨ J)
 
-private noncomputable def ww' (j : ℕ) := (ww i Hi j).val
+noncomputable def witness : tvar (tvar α') := ⟨ λ i, ⟨ λ j, @w i (j-i) ⟩ ⟩
 
 end witness
-include H SIM₀ SIM
+
+parameters Γ : cpred
+parameters H : Γ ⊢ SPEC₁ v o
+
+include SIM₀
+
+lemma init_in_w
+: Γ ⊢ ∀∀ w, ↑w ≃ witness ⟶ q;;⦃o,v⦄ ⟶ p;;⦃o,w⦄ :=
+begin
+  lifted_pred [witness,nat.sub_self,w] ,
+  intro Hq,
+  apply_epsilon_spec, simp,
+  intros, assumption,
+end
+
+include H SIM
+lemma J_inv_in_w
+: Γ ⊢ ∀∀ w, ↑w ≃ witness ⟶ ◻(J ;; ⦃o,v,w⦄) :=
+begin
+  lifted_pred keep,
+  intro i, simp [witness],
+  simp [nat.add_sub_cancel_left,w],
+  induction i with i,
+  { simp [w],
+    apply_epsilon_spec (SIM₀ _ _ _),
+    simp,
+    have := H.left.apply _ a, simp at this,
+    exact this },
+  { simp [w],
+    specialize @SIM _ (x + i ⊨ v) (x + i ⊨ o) (x + succ i ⊨ v) (x + succ i ⊨ o) ih_1,
+    apply_epsilon_spec (SIM _), simp,
+    replace H := (H.apply _ a).right i,
+    simp at H, simp [add_succ,H], },
+end
+
+lemma C_imp_A_in_w
+: Γ ⊢ ∀∀ w, ↑w ≃ witness ⟶ ◻(⟦ ⦃o,v⦄ <> C ⟧ ⟶ ⟦ ⦃o,w⦄ <> A ⟧) :=
+begin [temporal]
+  intros w Hw,
+  have := J_inv_in_w p q A C J SIM₀ @SIM v o Γ H,
+  replace this := this w Hw,
+  revert this,
+  apply henceforth_imp_henceforth ,
+  revert Hw w,
+  explicit {
+    simp, intros i,
+    have : σ ≤ σ + i, { simp [nat.zero_le], },
+    simp [witness,nat.add_sub_cancel_left,nat.succ_sub this,w],
+    intros hJ hC,
+    apply_epsilon_spec, simp,
+    intros, assumption, },
+end
 
 lemma simulation
 : Γ ⊢ ∃∃ w, SPEC₀ w o :=
-begin
-  simp [SPEC₀],
-  lifted_pred keep,
-  let w := ww' SIM₀ @SIM v o H _ a,
-  existsi (⟨ w ⟩ : tvar α'),
-  split,
-  intro i,
-  { simp,
-    generalize h : w (x + i) = z,
-    have h' : succ (x + i) > x,
-    { apply lt_succ_of_le, apply nat.le_add_right },
-    simp [w], rw [ww',ww], simp [dif_pos h'],
-    rw ← h,
-    apply_some_spec, simp, intros, assumption, },
-  { dsimp [w,ww'], rw ww, simp,
-    apply_some_spec,
-    simp, intros, assumption, },
+begin [temporal]
+  existsi witness p A J v o with Hw,
+  simp [SPEC₀], split,
+  { have := init_in_w p q A J SIM₀ v o Γ,
+    apply this witness₀ _ _, rw Hw,
+    apply H.left },
+  { have := C_imp_A_in_w p q A C J SIM₀ @SIM v o Γ H,
+    replace this := this witness₀ Hw,
+    have := H.right, revert this,
+    monotonicity only, apply this  }
 end
+
 omit H
 lemma simulation'
 : (∃∃ c, SPEC₁ c o) ⟹ (∃∃ a, SPEC₀ a o) :=
 begin [temporal]
   rw p_exists_p_imp,
   intros x h,
-  apply simulation SIM₀ @SIM _ _ h,
+  apply simulation p q A C J SIM₀ @SIM _ _ _ h,
 end
 
 end
@@ -168,7 +146,7 @@ parameters FIS₀ : ∃ σ, σ ⊨ p
 parameters FIS : ∀ σ, σ ⊨ J → ∃ σ', A σ σ'
 parameters INV : ∀ σ σ', σ ⊨ J → A σ σ' → σ' ⊨ J
 
-open classical
+open classical simulation
 
 include H₀ INV
 
@@ -208,179 +186,8 @@ begin
     have := FIS (w.down) hJ, revert this,
     apply exists_imp_exists' plift.up,
     introv hA, simp [A'], split,
-    { apply INV _ _ hJ hA  },
-    { apply hA } },
-  { simp [SPEC₁,C], }
-end
-
-end witness_construction
-
-section simulation
-
-parameters {α' : Type u} {β' : Type u₀} {γ' : Type u₁ }
-parameters {p : pred' (α'×γ')} {q : pred' (β'×γ')}
-parameters {A : act (α'×γ')} {C : act (β'×γ')}
-parameters {J : pred' (α'×β'×γ')}
-
-variables (x : tvar α') (y : tvar β') (z : tvar γ')
-
-def SPEC₀ (v : tvar α') (o : tvar γ') : cpred :=
-p ;; ⦃ o,v ⦄ ⋀
-◻⟦ ⦃o,v⦄ <> A ⟧
-
-def SPEC₁ (v : tvar β') (o : tvar γ') : cpred :=
-q ;; ⦃ o,v ⦄ ⋀
-◻⟦ ⦃o,v⦄ <> C ⟧
-
-parameter [inhabited α']
-parameter SIM₀ : ∀ v o, (v,o) ⊨ q → ∃ w, (w,o) ⊨ p ∧ (w,v,o) ⊨ J
-parameter SIM
-: ∀ {w v o} v' o',
-  (w,v,o) ⊨ J →
-  C (v,o) (v',o') →
-  ∃ w', A (w,o) (w',o') ∧
-        (w',v',o') ⊨ J
-
-parameters (v : tvar β') (o : tvar γ')
-
-parameters {Γ : cpred}
-parameters H : Γ ⊢ SPEC₁ v o
-
-section witness
-variables (i : ℕ) (Hi : i ⊨ Γ)
-include H Hi
-
-open classical
-
-private noncomputable def ww : Π j : ℕ, { w : α' // j ≥ i → (w,j ⊨ v,j ⊨ o) ⊨ J }
- | j :=
-if h : j > i then
-     have h₀ : j ≥ 1,
-       by { apply succ_le_of_lt,
-            apply nat.lt_of_le_of_lt (nat.zero_le i) h },
-     have h₁ : i ≤ j - 1,
-       by { rw ← add_le_to_le_sub _ ; assumption },
-     have Hdec : j - 1 < j,
-       by { apply nat.sub_lt_of_pos_le, apply zero_lt_one,
-            assumption },
-     let hw := (ww (j-1)).property h₁ in
-     have Hstep : C (j - 1 ⊨ v, j - 1 ⊨ o) (j ⊨ v, j ⊨ o),
-       begin
-         clear_except H Hi h₀ h₁ h, replace H := (H.apply _ Hi).right ((j-1) - i),
-         simp at H, rw [← nat.add_sub_assoc,nat.add_sub_cancel_left,← succ_sub] at H
-         ; apply H <|> assumption,
-       end,
-     let x := some (SIM (j ⊨ v) (j ⊨ o) hw Hstep) in
-     have h₁ : j ≥ i → (x, j ⊨ v, j ⊨ o) ⊨ J,
-       from assume _, (some_spec (SIM (j ⊨ v) (j ⊨ o) hw Hstep)).right,
-     ⟨x,h₁⟩
-else if h' : i ≤ j then
-     have h : i = j,
-       by { apply le_antisymm h', apply le_of_not_gt, assumption },
-     have h₀ : (j ⊨ v, j ⊨ o) ⊨ q,
-          begin
-            clear_except H Hi h,
-            have := H.left.apply _ Hi, simp at this,
-            subst i, apply this,
-          end,
-     let x₀ := some (SIM₀ (j ⊨ v) (j ⊨ o) h₀) in
-     have h₁ : j ≥ i → (x₀, j ⊨ v, j ⊨ o) ⊨ J,
-       from assume _, (some_spec (SIM₀ (j ⊨ v) (j ⊨ o) h₀)).right,
-     ⟨x₀,h₁⟩
-else
-  have h₁ : j ≥ i → (default α', j ⊨ v, j ⊨ o) ⊨ J,
-    by { intro, exfalso, apply h', assumption, },
-  ⟨default α',h₁⟩
-
-private noncomputable def ww' (j : ℕ) := (ww i Hi j).val
-
-end witness
-include H SIM₀ SIM
-
-lemma simulation
-: Γ ⊢ ∃∃ w, SPEC₀ w o :=
-begin
-  simp [SPEC₀],
-  lifted_pred keep,
-  let w := ww' SIM₀ @SIM v o H _ a,
-  existsi (⟨ w ⟩ : tvar α'),
-  split,
-  intro i,
-  { simp,
-    generalize h : w (x + i) = z,
-    have h' : succ (x + i) > x,
-    { apply lt_succ_of_le, apply nat.le_add_right },
-    simp [w], rw [ww',ww], simp [dif_pos h'],
-    rw ← h,
-    apply_some_spec, simp, intros, assumption, },
-  { dsimp [w,ww'], rw ww, simp,
-    apply_some_spec,
-    simp, intros, assumption, },
-end
-omit H
-lemma simulation'
-: (∃∃ c, SPEC₁ c o) ⟹ (∃∃ a, SPEC₀ a o) :=
-begin [temporal]
-  rw p_exists_p_imp,
-  intros x h,
-  apply simulation SIM₀ @SIM _ _ h,
-end
-
-end simulation
-
-section witness_construction
-
-parameters {α' : Sort u}
-parameters {p J : pred' α'}
-parameters {A : act α'}
-
-parameters H₀ : p ⟹ J
-parameters FIS₀ : ∃ σ, σ ⊨ p
-parameters FIS : ∀ σ, σ ⊨ J → ∃ σ', A σ σ'
-parameters INV : ∀ σ σ', σ ⊨ J → A σ σ' → σ' ⊨ J
-
-open classical
-
-include H₀ INV
-
-def A' : plift α' × unit → plift α' × unit → Prop :=
-A on (plift.down ∘ prod.fst)
-
-parameters [_inst : inhabited α']
-
-include FIS₀ FIS _inst
-lemma witness_construction
-: ⊩ ∃∃ v, p ;; v ⋀ ◻⟦ v <> A ⟧ :=
-begin
-  intro,
-  let o : tvar unit := ↑(),
-  let C : unit × unit → unit × unit → Prop := λ _ _, true,
-  let prj : var (plift α' × unit) α' := ↑(@plift.down α') ;; pair.fst,
-  let p' : pred' (plift α' × unit) := p ;; prj,
-  have _inst : inhabited (plift α') := ⟨ plift.up (default α') ⟩,
-  let J' : pred' (plift α' × unit × unit) := J ;; ↑(@plift.down α') ;; pair.fst,
-  have := @simulation _ _ _ p' (@True $ unit × unit) (A' H₀ INV) C J' _ _ _ o o Γ _,
-  begin [temporal]
-    revert this,
-    let f : tvar (plift α') → tvar α' := λ v, ↑(λ x : plift α', x.down) ;; v,
-    let SPEC := @SPEC₀ _ _ p' (A' H₀ INV),
-    let SPEC' := λ (v : tvar α'), p ;; v ⋀ ◻⟦ v <> A ⟧,
-    apply p_exists_imp_p_exists' (λ w, SPEC w o) SPEC' f,
-    intro, simp only [SPEC,f,SPEC',SPEC₀,p',prj,proj_assoc,pair.fst_mk,A'],
-    monotonicity, rw [action_on,coe_over_comp,proj_assoc,pair.fst_mk'],
-    refl,
-  end,
-  { intros,
-    revert FIS₀,
-    apply exists_imp_exists' plift.up,
-    introv h, split, simp [p',h],
-    simp [J'], apply ew_str H₀ _ h, },
-  { introv hJ hC, simp [J'] at hJ,
-    have := FIS (w.down) hJ, revert this,
-    apply exists_imp_exists' plift.up,
-    introv hA, simp [A'], split,
-    { apply INV _ _ hJ hA  },
-    { apply hA } },
+    { apply hA },
+    { apply INV _ _ hJ hA  } },
   { simp [SPEC₁,C], }
 end
 
@@ -388,117 +195,139 @@ end witness_construction
 
 namespace refinement
 section
-
+open fairness
 parameters {α' : Type u} {β' : Type u₀} {γ' : Type u₁ }
+parameters {evt : Type u₂}
 parameters {p : pred' (α'×γ')} {q : pred' (β'×γ')}
-parameters {A : ℕ → act (α'×γ')} {C : ℕ → act (β'×γ')}
-parameters {g : ℕ → pred' (α'×γ')} {g' : ℕ → pred' (β'×γ')}
-parameters {J : pred' (α'×β'×γ')}
-
-variables (x : tvar α') (y : tvar β') (z : tvar γ')
+parameters (A : evt → act (α'×γ')) (C : evt → act (β'×γ'))
+parameters {cs₀ fs₀ : evt → pred' (α'×γ')} {cs₁ fs₁ : evt → pred' (β'×γ')}
+parameters (J : pred' (α'×β'×γ'))
 
 def SPEC₀ (v : tvar α') (o : tvar γ') : cpred :=
 p ;; ⦃ o,v ⦄ ⋀
 ◻(∃∃ i, ⟦ ⦃o,v⦄ <> A i ⟧) ⋀
-∀∀ i : ℕ, wf (g i ;; ⦃o,v⦄) ⟦ ⦃o,v⦄ <> A i ⟧
+∀∀ i, sched (cs₀ i ;; ⦃o,v⦄) (fs₀ i ;; ⦃o,v⦄) ⟦ ⦃o,v⦄ <> A i ⟧
 
 def SPEC₁ (v : tvar β') (o : tvar γ') : cpred :=
 q ;; ⦃ o,v ⦄ ⋀
-◻⟦ ⦃o,v⦄ <> C ⟧
+◻(∃∃ i, ⟦ ⦃o,v⦄ <> C i ⟧) ⋀
+∀∀ i, sched (cs₁ i ;; ⦃o,v⦄) (fs₁ i ;; ⦃o,v⦄) ⟦ ⦃o,v⦄ <> C i ⟧
+
+def SPEC₂ (v : tvar β') (o : tvar γ') (s : tvar evt) : cpred :=
+q ;; ⦃ o,v ⦄ ⋀
+◻(∃∃ i, s ≃ ↑i ⋀ ⟦ ⦃o,v⦄ <> C i ⟧) ⋀
+∀∀ i, sched (cs₁ i ;; ⦃o,v⦄) (fs₁ i ;; ⦃o,v⦄) (s ≃ ↑i ⋀ ⟦ ⦃o,v⦄ <> C i ⟧)
 
 parameter [inhabited α']
 parameter SIM₀ : ∀ v o, (v,o) ⊨ q → ∃ w, (w,o) ⊨ p ∧ (w,v,o) ⊨ J
 parameter SIM
-: ∀ {w v o} v' o',
+: ∀ w v o v' o' e,
   (w,v,o) ⊨ J →
-  C (v,o) (v',o') →
-  ∃ w', A (w,o) (w',o') ∧
+  C e (v,o) (v',o') →
+  ∃ w', A e (w,o) (w',o') ∧
         (w',v',o') ⊨ J
 
-parameters (v : tvar β') (o : tvar γ')
+parameters (v : tvar β') (o : tvar γ') (sch : tvar evt)
 
-parameters {Γ : cpred}
-parameters H : Γ ⊢ SPEC₁ v o
+parameters (Γ : cpred)
+parameters H : Γ ⊢ SPEC₂ v o sch
 
-section witness
-variables (i : ℕ) (Hi : i ⊨ Γ)
-include H Hi
+def cv := ⦃o,v⦄
+variable Hdelay : Γ ⊢ ∀∀ e w, cs₀ e;;⦃o,w⦄ ⋀ fs₀ e;;⦃o,w⦄ ~> cs₁ e;;cv
+variable Hresched : Γ ⊢ ∀∀ e w, cs₀ e;;⦃o,w⦄ ⋀ fs₀ e;;⦃o,w⦄ ~> fs₁ e;;cv
+variable Hstable : Γ ⊢ ∀∀ e w, ◻◇(cs₁ e;;cv) ⟶ ◇◻(cs₁ e;;cv) ⋁ ◻◇-(cs₀ e;;⦃o,w⦄)
 
-open classical
+open simulation (witness init_in_w C_imp_A_in_w) prod temporal.prod
 
-private noncomputable def ww : Π j : ℕ, { w : α' // j ≥ i → (w,j ⊨ v,j ⊨ o) ⊨ J }
- | j :=
-if h : j > i then
-     have h₀ : j ≥ 1,
-       by { apply succ_le_of_lt,
-            apply nat.lt_of_le_of_lt (nat.zero_le i) h },
-     have h₁ : i ≤ j - 1,
-       by { rw ← add_le_to_le_sub _ ; assumption },
-     have Hdec : j - 1 < j,
-       by { apply nat.sub_lt_of_pos_le, apply zero_lt_one,
-            assumption },
-     let hw := (ww (j-1)).property h₁ in
-     have Hstep : C (j - 1 ⊨ v, j - 1 ⊨ o) (j ⊨ v, j ⊨ o),
-       begin
-         clear_except H Hi h₀ h₁ h, replace H := (H.apply _ Hi).right ((j-1) - i),
-         simp at H, rw [← nat.add_sub_assoc,nat.add_sub_cancel_left,← succ_sub] at H
-         ; apply H <|> assumption,
-       end,
-     let x := some (SIM (j ⊨ v) (j ⊨ o) hw Hstep) in
-     have h₁ : j ≥ i → (x, j ⊨ v, j ⊨ o) ⊨ J,
-       from assume _, (some_spec (SIM (j ⊨ v) (j ⊨ o) hw Hstep)).right,
-     ⟨x,h₁⟩
-else if h' : i ≤ j then
-     have h : i = j,
-       by { apply le_antisymm h', apply le_of_not_gt, assumption },
-     have h₀ : (j ⊨ v, j ⊨ o) ⊨ q,
-          begin
-            clear_except H Hi h,
-            have := H.left.apply _ Hi, simp at this,
-            subst i, apply this,
-          end,
-     let x₀ := some (SIM₀ (j ⊨ v) (j ⊨ o) h₀) in
-     have h₁ : j ≥ i → (x₀, j ⊨ v, j ⊨ o) ⊨ J,
-       from assume _, (some_spec (SIM₀ (j ⊨ v) (j ⊨ o) h₀)).right,
-     ⟨x₀,h₁⟩
-else
-  have h₁ : j ≥ i → (default α', j ⊨ v, j ⊨ o) ⊨ J,
-    by { intro, exfalso, apply h', assumption, },
-  ⟨default α',h₁⟩
+def Next_a :=
+λ σ σ', ∃ e, A e σ σ'
 
-private noncomputable def ww' (j : ℕ) := (ww i Hi j).val
+def Next_c :=
+λ σ σ' : (evt × β') × γ', ∃ e, σ.1.1 = e ∧ (C e on map_left snd) σ σ'
 
-end witness
-include H SIM₀ SIM
+section J
+parameter evt
+def J' : pred' (α' × (evt × β') × γ') :=
+J ;; ((prod.map_right $ prod.map_left prod.snd) : (α' × (evt × β') × γ') → (α' × β' × γ'))
 
-lemma simulation
-: Γ ⊢ ∃∃ w, SPEC₀ w o :=
+parameter q
+def q' : pred' ((evt × β') × γ') :=
+q ;; (prod.map_left prod.snd : (evt × β') × γ' → β' × γ')
+
+end J
+
+section Simulation_POs
+include SIM₀
+lemma SIM₀' (v : evt × β') (o : γ')
+  (h : (v, o) ⊨ q')
+: (∃ (w : α'), (w, o) ⊨ p ∧ (w, v, o) ⊨ J') :=
 begin
-  simp [SPEC₀],
-  lifted_pred keep,
-  let w := ww' SIM₀ @SIM v o H _ a,
-  existsi (⟨ w ⟩ : tvar α'),
-  split,
-  intro i,
-  { simp,
-    generalize h : w (x + i) = z,
-    have h' : succ (x + i) > x,
-    { apply lt_succ_of_le, apply nat.le_add_right },
-    simp [w], rw [ww',ww], simp [dif_pos h'],
-    rw ← h,
-    apply_some_spec, simp, intros, assumption, },
-  { dsimp [w,ww'], rw ww, simp,
-    apply_some_spec,
-    simp, intros, assumption, },
+  simp [q',prod.map_left] at h,
+  specialize SIM₀ v.2 o h,
+  revert SIM₀, intros_mono,
+  simp [J'],
 end
-omit H
-lemma simulation'
-: (∃∃ c, SPEC₁ c o) ⟹ (∃∃ a, SPEC₀ a o) :=
+omit SIM₀
+include SIM
+lemma SIM' (w : α') (v : evt × β') (o : γ') (v' : evt × β') (o' : γ')
+  (h₀ : (w, v, o) ⊨ J')
+  (h₁ : Next_c (v, o) (v', o'))
+: (∃ (w' : α'), Next_a (w, o) (w', o') ∧ (w', v', o') ⊨ J') :=
+sorry
+omit SIM
+lemma H'
+: Γ ⊢ simulation.SPEC₁ q' Next_c ⦃v,sch⦄ o :=
+sorry
+
+end Simulation_POs
+
+include H SIM₀ SIM Hstable Hdelay Hresched
+
+lemma one_to_one
+: Γ ⊢ ∃∃ w, SPEC₀ w o :=
 begin [temporal]
-  rw p_exists_p_imp,
-  intros x h,
-  apply simulation SIM₀ @SIM _ _ h,
+  -- type_check witness p (Next_a A) J' ⦃sch,v⦄ o ,
+  existsi witness p (Next_a A) (J' evt J) ⦃v,sch⦄ o with Hw,
+  -- existsi witness p (Next_a A) J v o with Hw,
+  have this := H, revert this,
+  dsimp [SPEC₀,SPEC₁],
+  -- type_check ctx_imp_entails_p_imp _ _,
+  replace SIM := SIM' A C J SIM,
+  replace SIM₀ := SIM₀' _ SIM₀,
+  replace H := H' evt q C v o sch Γ,
+  apply ctx_p_and_p_imp_p_and' _ _,
+  apply ctx_p_and_p_imp_p_and' _ _,
+  { clear_except SIM₀ Hw H,
+    have := init_in_w p (q' evt q) (Next_a A) (J' evt J) SIM₀ ⦃v,sch⦄ o Γ,
+    intro Hq,
+    apply this witness₀ Hw _,
+    simp [q',proj_assoc], apply Hq, },
+  { clear_except SIM SIM₀ Hw H,
+    have := C_imp_A_in_w p (q' evt q) (Next_a A) (Next_c C) (J' evt J) SIM₀ SIM ⦃v,sch⦄ o Γ H,
+    { replace this := this witness₀ Hw,
+      monotonicity only,
+      simp [exists_action],
+      intros e h₀ h₁, apply this _,
+      simp [Next_c],
+      suffices : ⟦ ⦃o,⦃v,sch⦄⦄ <> λ (σ σ' : (evt × β') × γ'), ((λ s s', s = e) on (prod.fst ∘ prod.fst)) σ σ' ∧ (C e on map_left snd) σ σ' ⟧,
+      revert this, action
+      { simp [function.on_fun],
+      intros, subst e, assumption, },
+      rw ← action_and_action, simp,
+      rw [action_on,action_on,coe_over_comp,proj_assoc,← init_eq_action,coe_eq],
+      simp, split ; assumption } },
+  { intros h i,
+    apply replacement Γ _ _ _ _ (h i),
+    apply Hdelay i _,
+    apply Hstable i _,
+    admit,
+    apply Hresched i _, },
 end
+
+omit H
+lemma data_refinement'
+: (∃∃ c, SPEC₁ c o) ⟹ (∃∃ a, SPEC₀ a o) :=
+sorry
 
 end
 end refinement
