src/temporal_logic/pair.lean
@@ -1,0 +1,65 @@
+import temporal_logic.lemmas
+
+universe variables u u₀ u₁ u₂
+
+local attribute [-simp] or.comm or.left_comm or.assoc and.comm and.left_comm and.assoc
+
+namespace temporal
+open predicate
+
+section pair
+
+variables {α' : Type u} {β' : Type u₀} {γ' : Type u₁}
+variables (x : tvar α') (y : tvar β') (z : tvar γ')
+
+def pair : tvar (α' × β') :=
+lifted₂ prod.mk x y
+
+notation `⦃` x `,` l:(foldl `,` (h t, pair h t) x `⦄`)  := l
+
+@[simp]
+lemma pair_model (i : ℕ) :
+i ⊨ ⦃x,y⦄ = (i ⊨ y,i ⊨ x) :=
+by { cases x, cases y, refl }
+
+@[reducible]
+def pair.fst : var (α' × β') α' :=
+↑(@prod.fst α' β')
+
+@[simp]
+def pair.fst_mk (x : tvar α') (y : tvar β')
+: pair.fst ;; ⦃y,x⦄ = x :=
+by lifted_pred
+
+@[simp]
+def pair.fst_mk' (x : tvar α') (y : tvar β')
+: ↑(@prod.fst α' β') ;; ⦃y,x⦄ = x :=
+pair.fst_mk _ _
+
+@[simp]
+def pair.snd_mk' (x : tvar α') (y : tvar β')
+: ↑(@prod.snd α' β') ;; ⦃y,x⦄ = y :=
+by lifted_pred
+
+@[simp]
+def prod.map_left {α β γ} (f : α → β) : α × γ → β × γ
+ | (x,y) := (f x, y)
+
+@[simp]
+def prod.map_right {α β γ} (f : β → γ) : α × β → α × γ
+ | (x,y) := (x,f y)
+open temporal.prod
+
+@[simp]
+lemma map_right_proj_pair (f : α' → γ')
+: ((@map_right β' _ _ f) : var (β' × α') (β' × γ')) ;; ⦃x,y⦄ = ⦃↑f ;; x, y⦄ :=
+by funext i ; simp [map_right]
+
+@[simp]
+lemma map_left_proj_pair (f : α' → γ')
+: ((@map_left _ _ β' f) : var (α' × β') (γ' × β')) ;; ⦃y,x⦄ = ⦃y, ↑f ;; x⦄ :=
+by funext i ; simp [map_left]
+
+end pair
+
+end temporal
